\begin{answer}
  Let's compute the posterior probability $p(y=1 | x)$ for the (GDA) model.

  Using Bayes rule we have:

  \begin{equation}
    p(y=1| x; \phi, \mu_0,\mu_1,\Sigma) = \dfrac{p(y=1)p(x\;|\;y=1)}
    {p(y=1)p(x\;|\;y=1) + p(y=0)p(x\;|\;y=0)}
  \end{equation}

  We use the definition of each distribution and we factorized by
  the marginalisation constant.

  \begin{equation}
    p(y=1\;|\; x) = \dfrac{\exp(G_{u_1}(x))}{
    \exp(G_{u_0}(x)) + \exp(G_{u_1}(x))}
  \end{equation}

  Where $G_u(x) = \dfrac{-1}{2}(x - u)^T\Sigma^{-1}(x-u)$


  \begin{equation}
    p(y=1|x) = \dfrac{1}{ 1 + \exp(G_{u_1}(x)- G_{u2}(x))}
  \end{equation}

  Finally we compute the difference between the two Gaussians
  \newcommand{\precision}{\Sigma^{-1}}
  \begin{equation}
    G_{u_1}(x) - G_{u_0}(x) = x^T\precision x -2u_1^T\precision
    x -u_1\precision u_1 - x^T\precision x +2u_0^T\precision x -
    u_0\precision u_0
  \end{equation}

  \begin{equation}
    G_{u_1} - G_{u_0} = 2(u_0 - u_1)^T\precision x + (u_0 -
    u_1)^T\precision (u_0 - u_1)
  \end{equation}
\end{answer}
